common/SmallstepClosed.v
@@ -1,0 +1,134 @@
+Require Import Relations.
+Require Import Wellfounded.
+Require Import Coqlib.
+Require Import Errors.
+Require Import Events.
+Require Import Globalenvs.
+Require Import LanguageInterface.
+Require Import Integers.
+Require Import Invariant.
+Require Import SmallstepLinkingSafe Smallstep.
+
+Import Values Maps Memory AST.
+
+Set Implicit Arguments.
+
+(* Definitions. *)
+
+Record semantics := ClosedSemantics_gen {
+  state: Type;
+  genvtype: Type;
+  step : genvtype -> state -> trace -> state -> Prop;
+  initial_state: state -> Prop;
+  final_state: state -> val -> Prop; (* For closed safety, we should make
+  the return value to be val instead of int *)
+  globalenv: genvtype;
+  symbolenv: Genv.symtbl
+}.
+
+Declare Scope closed_smallstep_scope.
+
+Notation " 'Step' L " := (step L (globalenv L)) (at level 1) : closed_smallstep_scope.
+Notation " 'Star' L " := (star (step L) (globalenv L)) (at level 1) : closed_smallstep_scope.
+Notation " 'Plus' L " := (plus (step L) (globalenv L)) (at level 1) : closed_smallstep_scope.
+Notation " 'Forever_silent' L " := (forever_silent (step L) (globalenv L)) (at level 1) : closed_smallstep_scope.
+Notation " 'Forever_reactive' L " := (forever_reactive (step L) (globalenv L)) (at level 1) : closed_smallstep_scope.
+Notation " 'Nostep' L " := (nostep (step L) (globalenv L)) (at level 1) : closed_smallstep_scope.
+Notation " 'Eventually' L " := (eventually (step L) (final_state L) (globalenv L)) (at level 1) : closed_smallstep_scope.
+Open Scope closed_smallstep_scope.
+
+
+(* Closing open semantics. *)
+
+Section CLOSE_SEMANTICS.
+
+Variable liA liB : language_interface.
+Variable s : Smallstep.semantics liA liB.
+Variable se : Genv.symtbl.
+Variable init_q : program unit unit -> option (query liB). (* a function from
+program to initial query *)
+Variable final_r : reply liB -> val. (* a function from reply to return value *)
+
+Definition close_semantics :=
+  let lts := Smallstep.activate s se in
+  {|
+    state := Smallstep.state s;
+    genvtype := Smallstep.genvtype lts;
+    step := Smallstep.step lts;
+    initial_state :=
+      match init_q (skel s) with
+      | Some q =>
+          Smallstep.initial_state lts q
+      | None => fun _ => False
+      end;
+    final_state := fun state retval =>
+                     exists r, Smallstep.final_state lts state r /\ retval = final_r r;
+    globalenv := Smallstep.globalenv lts;
+    symbolenv := se;
+  |}.
+
+End CLOSE_SEMANTICS.
+
+Definition safe (L: semantics) (s: state L) : Prop :=
+  forall s',
+  Star L s E0 s' ->
+  (exists r, final_state L s' r)
+  \/ (exists t, exists s'', Step L s' t s'').
+
+(* Closed safety is defined as reachable safety *)
+Definition closed_safety (L: semantics) : Prop :=
+  forall s, initial_state L s -> safe L s.
+
+Section CLOSED_SAFE.
+
+Variable liA liB : language_interface.
+Variable IB: invariant liB.
+Variable s : Smallstep.semantics liA liB.
+Variable se : Genv.symtbl.
+Variable init_q : program unit unit -> option (query liB). (* a function from
+program to initial query *)
+Variable final_r : reply liB -> val. (* a function from reply to return value *)
+
+Definition lts := (Smallstep.activate s se).
+Definition L := close_semantics s se init_q final_r.
+
+Hypothesis VSE: Genv.valid_for (skel s) se.
+
+(* The query must satisfy the pre-condition if it can be
+constructed. Most of the time we just set the query_inv and symtbl_inv
+to be True for the main function *)
+Hypothesis QINV: forall q, init_q (skel s) = Some q ->
+                      valid_query lts q = true
+                      /\ (exists w, query_inv IB w q
+                              /\ symtbl_inv IB w se).
+
+
+Theorem closed_open_safety_sound:
+  module_type_safe inv_bot IB s SIF ->
+  closed_safety L.
+Proof.
+  intros [(inv & SAFE)].
+  red. intros inits INIT.
+  simpl in INIT.
+  destruct (init_q (skel s)) eqn: INIQ; try contradiction.
+  exploit QINV; eauto. intros (VQ & (w & HQ & SYM)).
+  specialize (SAFE se w SYM VSE).
+
+  exploit @initial_preserves_progress; eauto.
+  intros (inits' & INIT' & INIT_SAFE).
+  specialize (INIT_SAFE inits INIT).
+  red. intros s' STAR.
+  exploit @lts_preserves_progress_internal_safe; eauto.
+  intros [(r & FINAL)|[(q1 & EXT)|(t1 & s1 & STEP1)]]; eauto.
+  - left. simpl.
+    exists (final_r r), r. eauto.
+  - exploit @lts_preserves_progress_star. eauto.
+    simpl in STAR. eauto. auto.
+    intros SINV.
+    exploit @external_preserves_progress; eauto.
+    intros (wA & A1 & A2 & A3). inv A2.
+Qed.
+
+
+End CLOSED_SAFE.
+
